Prove safey in another definition

Isabelle/ConsensusSafety.thy
@@ -112,8 +112,7 @@ proof-
   and "finite \<sigma>_set"
   and "is_faults_lt_threshold (\<Union> \<sigma>_set)"
   hence "\<exists>\<sigma>\<in>\<Sigma>t. \<sigma> \<in> \<Inter> {futures \<sigma> | \<sigma>. \<sigma> \<in> \<sigma>_set}"
-    using n_party_common_futures_exists
-    by (simp add: \<open>finite \<sigma>_set\<close> \<open>is_faults_lt_threshold (\<Union>\<sigma>_set)\<close> \<sigma>_set)
+    using n_party_common_futures_exists by simp
   hence "\<exists>\<sigma>\<in>\<Sigma>t. \<forall>s\<in>\<sigma>_set. \<sigma> \<in> futures s"
     by blast
   hence "\<exists>\<sigma>\<in>\<Sigma>t. (\<forall>s\<in>\<sigma>_set. \<sigma> \<in> futures s) \<and> (\<forall>s\<in>\<sigma>_set. \<sigma> \<in> futures s \<longrightarrow> (\<forall>p. state_property_is_decided (p,s) \<longrightarrow> state_property_is_decided (p,\<sigma>)))"
@@ -230,6 +229,37 @@ proof -
   thus
     "consensus_value_properties_are_consistent (\<Union> {consensus_value_property_decisions \<sigma> | \<sigma>. \<sigma> \<in> \<sigma>_set})"
     by simp
+qed
+
+fun consensus_value_property_not :: "consensus_value_property \<Rightarrow> consensus_value_property"
+  where
+    "consensus_value_property_not p = (\<lambda>c. (\<not> p c))"
+
+theorem (in Protocol) n_party_safety :
+  "\<forall> \<sigma>_set. \<sigma>_set \<subseteq> \<Sigma>t
+  \<longrightarrow> finite \<sigma>_set
+  \<longrightarrow> is_faults_lt_threshold (\<Union> \<sigma>_set)
+  \<longrightarrow> (\<forall> \<sigma> \<sigma>' p. {\<sigma>, \<sigma>'} \<subseteq> \<sigma>_set \<and> p \<in> consensus_value_property_decisions \<sigma> \<longrightarrow> consensus_value_property_not p \<notin> consensus_value_property_decisions \<sigma>')"
+  apply (rule, rule, rule, rule, rule, rule, rule, rule)
+proof -
+  fix \<sigma>_set \<sigma> \<sigma>' p
+  assume "\<sigma>_set \<subseteq> \<Sigma>t" and "finite \<sigma>_set" and "is_faults_lt_threshold (\<Union>\<sigma>_set)" and "{\<sigma>, \<sigma>'} \<subseteq> \<sigma>_set \<and> p \<in> consensus_value_property_decisions \<sigma>" 
+  hence "\<exists> \<sigma>. \<sigma> \<in> \<Sigma>t \<and> \<sigma> \<in> \<Inter> {futures \<sigma> | \<sigma>. \<sigma> \<in> \<sigma>_set}"
+    using n_party_common_futures_exists by meson
+  then obtain \<sigma>'' where "\<sigma>'' \<in> \<Sigma>t \<and> \<sigma>'' \<in> \<Inter> {futures \<sigma> | \<sigma>. \<sigma> \<in> \<sigma>_set}" by auto
+  hence "state_property_is_decided (naturally_corresponding_state_property p, \<sigma>'')" 
+    using \<open>{\<sigma>, \<sigma>'} \<subseteq> \<sigma>_set \<and> p \<in> consensus_value_property_decisions \<sigma>\<close> consensus_value_property_decisions_def consensus_value_property_is_decided_def 
+    using \<open>\<sigma>_set \<subseteq> \<Sigma>t\<close> forward_consistency by fastforce
+  have "\<sigma>'' \<in> futures \<sigma>'" 
+    using \<open>\<sigma>'' \<in> \<Sigma>t \<and> \<sigma>'' \<in> \<Inter> {futures \<sigma> | \<sigma>. \<sigma> \<in> \<sigma>_set}\<close> \<open>{\<sigma>, \<sigma>'} \<subseteq> \<sigma>_set \<and> p \<in> consensus_value_property_decisions \<sigma>\<close>
+    by auto
+  hence "\<not> state_property_is_decided (state_property_not (naturally_corresponding_state_property p), \<sigma>')"
+      (* NOTE: About the non-deterministicity, should we define this as safety? *)
+      using backword_consistency \<open>state_property_is_decided (naturally_corresponding_state_property p, \<sigma>'')\<close>
+      using \<open>\<sigma>'' \<in> \<Sigma>t \<and> \<sigma>'' \<in> \<Inter>_Collect (futures \<sigma>) (\<sigma> \<in> \<sigma>_set)\<close> \<open>\<sigma>_set \<subseteq> \<Sigma>t\<close> \<open>{\<sigma>, \<sigma>'} \<subseteq> \<sigma>_set \<and> p \<in> consensus_value_property_decisions \<sigma>\<close> by auto  
+  then show "consensus_value_property_not p \<notin> consensus_value_property_decisions \<sigma>'"
+    apply (simp add: consensus_value_property_decisions_def consensus_value_property_is_decided_def naturally_corresponding_state_property_def state_property_is_decided_def)
+    using \<Sigma>t_def estimates_are_non_empty futures_def by fastforce   
 qed
 
 end
